serialize string, tagged

src/cddl/pulse/CDDL.Pulse.Serialize.Misc.fst
@@ -162,3 +162,265 @@ fn impl_serialize_int_range_neg_int64
     0sz
   }
 }
+
+inline_for_extraction noextract [@@noextract_to "krml";
+  FStar.Tactics.postprocess_with (fun _ -> FStar.Tactics.norm [delta; zeta; iota; primops]; FStar.Tactics.trefl ())
+]
+let pow2_64_m1 : U64.t = U64.uint_to_t (pow2 64 - 1)
+
+let pow2_64_m1_eq : squash (U64.v pow2_64_m1 == pow2 64 - 1) = _ by (
+  FStar.Tactics.norm [delta; zeta; iota; primops];
+  FStar.Tactics.trefl ()
+)
+
+inline_for_extraction noextract [@@noextract_to "krml"]
+fn impl_serialize_bstr
+  (#ty: Type u#0)
+  (#vmatch: perm -> ty -> cbor -> slprop)
+  (cbor_det_serialize: cbor_det_serialize_t vmatch)
+  (cbor_mk_string: mk_string_t vmatch)
+  (freeable: Ghost.erased bool)
+: impl_serialize #_ #_ #_ spec_bstr #_ (rel_slice_of_seq freeable)
+=
+  (c: _)
+  (#v: _)
+  (out: _)
+{
+  let _ : squash (SZ.fits_u64) = assume (SZ.fits_u64);
+  unfold (rel_slice_of_seq freeable c v);
+  S.pts_to_len c.s;
+  let len = S.len c.s;
+  if (SZ.lte len (SZ.uint64_to_sizet pow2_64_m1)) {
+    let g = Ghost.hide (pack (CString cbor_major_type_byte_string v));
+    Cbor.cbor_det_serialize_parse g;
+    let x = cbor_mk_string cbor_major_type_byte_string c.s;
+    let ser = cbor_det_serialize x out;
+    Trade.elim _ _;
+    fold (rel_slice_of_seq freeable c v);
+    match ser {
+      None -> {
+        0sz
+      }
+      Some sz -> {
+        sz
+      }
+    }
+  } else {
+    fold (rel_slice_of_seq freeable c v);
+    0sz
+  }
+}
+
+inline_for_extraction noextract [@@noextract_to "krml"]
+fn impl_serialize_tstr
+  (#ty: Type u#0)
+  (#vmatch: perm -> ty -> cbor -> slprop)
+  (cbor_utf8_correct: impl_utf8_correct_t)
+  (cbor_det_serialize: cbor_det_serialize_t vmatch)
+  (cbor_mk_string: mk_string_t vmatch)
+  (freeable: Ghost.erased bool)
+: impl_serialize #_ #_ #_ spec_tstr #_ (rel_slice_of_seq freeable)
+=
+  (c: _)
+  (#v: _)
+  (out: _)
+{
+  let _ : squash (SZ.fits_u64) = assume (SZ.fits_u64);
+  unfold (rel_slice_of_seq freeable c v);
+  S.pts_to_len c.s;
+  let len = S.len c.s;
+  if (SZ.lte len (SZ.uint64_to_sizet pow2_64_m1)) {
+    let correct = cbor_utf8_correct c.s;
+    if (correct) {
+      let g = Ghost.hide (pack (CString cbor_major_type_text_string v));
+      Cbor.cbor_det_serialize_parse g;
+      let x = cbor_mk_string cbor_major_type_text_string c.s;
+      let ser = cbor_det_serialize x out;
+      Trade.elim _ _;
+      fold (rel_slice_of_seq freeable c v);
+      match ser {
+        None -> {
+          0sz
+        }
+        Some sz -> {
+          sz
+        }
+      }
+    } else {
+      fold (rel_slice_of_seq freeable c v);
+      0sz
+    }
+  } else {
+    fold (rel_slice_of_seq freeable c v);
+    0sz
+  }
+}
+
+inline_for_extraction noextract [@@noextract_to "krml"]
+fn impl_serialize_str_size
+  (#ty: Type u#0)
+  (#vmatch: perm -> ty -> cbor -> slprop)
+  (cbor_utf8_correct: impl_utf8_correct_t)
+  (cbor_det_serialize: cbor_det_serialize_t vmatch)
+  (cbor_mk_string: mk_string_t vmatch)
+  (freeable: Ghost.erased bool)
+  (mt: major_type_byte_string_or_text_string)
+  (lo: U64.t)
+  (hi: U64.t)
+: impl_serialize #_ #_ #_ (spec_str_size mt lo hi) #_ (rel_slice_of_seq freeable)
+=
+  (c: _)
+  (#v: _)
+  (out: _)
+{
+  let _ : squash (SZ.fits_u64) = assume (SZ.fits_u64);
+  unfold (rel_slice_of_seq freeable c v);
+  S.pts_to_len c.s;
+  let len = S.len c.s;
+  fold (rel_slice_of_seq freeable c v);
+  if (SZ.lte (SZ.uint64_to_sizet lo) len && SZ.lte len (SZ.uint64_to_sizet hi)) {
+    if (mt = cbor_major_type_byte_string) {
+      impl_serialize_bstr cbor_det_serialize cbor_mk_string freeable c out;
+    } else {
+      impl_serialize_tstr cbor_utf8_correct cbor_det_serialize cbor_mk_string freeable c out;
+    }
+  } else {
+    0sz
+  }
+}
+
+inline_for_extraction noextract [@@noextract_to "krml"]
+fn impl_serialize_simple
+  (#ty: Type u#0)
+  (#vmatch: perm -> ty -> cbor -> slprop)
+  (cbor_det_serialize: cbor_det_serialize_t vmatch)
+  (cbor_mk_simple: mk_simple_t vmatch)
+  (cbor_elim_simple: elim_simple_t vmatch)
+: impl_serialize #_ #_ #_ spec_simple #_ (rel_pure U8.t)
+=
+  (c: _)
+  (#v: _)
+  (out: _)
+{
+  unfold (rel_pure U8.t c v);
+  assert (pure (c == Ghost.reveal v)); // FIXME: WHY WHY WHY?
+  fold (rel_pure U8.t c v);
+  if (simple_value_wf c) {
+    let g = Ghost.hide (pack (CSimple c));
+    Cbor.cbor_det_serialize_parse g;
+    let x = cbor_mk_simple c;
+    let ser = cbor_det_serialize x out;
+    cbor_elim_simple x;
+    match ser {
+      None -> {
+        0sz
+      }
+      Some sz -> {
+        sz
+      }
+    }
+  } else {
+    0sz
+  }
+}
+
+inline_for_extraction noextract [@@noextract_to "krml"]
+fn impl_serialize_bool
+  (#ty: Type u#0)
+  (#vmatch: perm -> ty -> cbor -> slprop)
+  (cbor_det_serialize: cbor_det_serialize_t vmatch)
+  (cbor_mk_simple: mk_simple_t vmatch)
+  (cbor_elim_simple: elim_simple_t vmatch)
+: impl_serialize #_ #_ #_ spec_bool #_ (rel_pure bool)
+=
+  (c: _)
+  (#v: _)
+  (out: _)
+{
+  unfold (rel_pure bool c v);
+  assert (pure (c == Ghost.reveal v)); // FIXME: WHY WHY WHY?
+  fold (rel_pure bool c v);
+  let c' = c; // FIXME: need `norewrite` on `if`
+  if (c') {
+    fold (rel_pure U8.t simple_value_true simple_value_true);
+    let res = impl_serialize_simple cbor_det_serialize cbor_mk_simple cbor_elim_simple simple_value_true out;
+    unfold (rel_pure U8.t simple_value_true simple_value_true);
+    res
+  } else {
+    fold (rel_pure U8.t simple_value_false simple_value_false);
+    let res = impl_serialize_simple cbor_det_serialize cbor_mk_simple cbor_elim_simple simple_value_false out;
+    unfold (rel_pure U8.t simple_value_false simple_value_false);
+    res
+  }
+}
+
+#push-options "--z3rlimit 32"
+
+inline_for_extraction noextract [@@noextract_to "krml"]
+fn impl_serialize_tagged_none
+    (cbor_det_serialize_tag: cbor_det_serialize_tag_t)
+    (#[@@@erasable]t1: Ghost.erased typ)
+    (#[@@@erasable]tgt1: Type0)
+    (#[@@@erasable] inj1: Ghost.erased bool)
+    (#[@@@erasable]ps1: Ghost.erased (spec t1 tgt1 inj1))
+    (#impl_tgt1: Type0)
+    (#[@@@erasable]r1: rel impl_tgt1 tgt1)
+    (i1: impl_serialize ps1 r1)
+: impl_serialize #_ #_ #_ (spec_tag_none ps1) #_ (rel_pair (rel_pure U64.t) r1)
+=
+    (c: _)
+    (#v: _)
+    (out: _)
+{
+  norewrite let (ctag, cpayload) = c;
+  Trade.rewrite_with_trade
+    (rel_pair (rel_pure U64.t) r1 c v)
+    (pure (ctag == fst v) ** r1 cpayload (snd v));
+  let tsz = cbor_det_serialize_tag ctag out;
+  Classical.forall_intro (Cbor.cbor_det_serialize_tag_correct ctag);
+  if (tsz = 0sz) {
+    Trade.elim _ _;
+    0sz
+  } else {
+    let (_, out2) = S.split out tsz;
+    let psz = i1 cpayload out2;
+    S.join _ _ out;
+    S.pts_to_len out;
+    Trade.elim _ _;
+    if (psz = 0sz) {
+      0sz
+    } else {
+      (SZ.add tsz psz)
+    }
+  }
+}
+
+#pop-options
+
+inline_for_extraction noextract [@@noextract_to "krml"]
+fn impl_serialize_tagged_some
+    (cbor_det_serialize_tag: cbor_det_serialize_tag_t)
+    (tag: U64.t)
+    (#[@@@erasable]t1: Ghost.erased typ)
+    (#[@@@erasable]tgt1: Type0)
+    (#[@@@erasable] inj1: Ghost.erased bool)
+    (#[@@@erasable]ps1: Ghost.erased (spec t1 tgt1 inj1))
+    (#impl_tgt1: Type0)
+    (#[@@@erasable]r1: rel impl_tgt1 tgt1)
+    (i1: impl_serialize ps1 r1)
+: impl_serialize #_ #_ #_ (spec_tag_some tag ps1) #_ r1
+=
+    (c: _)
+    (#v: _)
+    (out: _)
+{
+  let c' = (tag, c);
+  rel_pair_eq (rel_pure U64.t) r1 tag c tag v;
+  rel_pure_eq tag tag;
+  Trade.rewrite_with_trade
+    (pure (tag == tag) ** r1 c v)
+    (rel_pair (rel_pure U64.t) r1 c' (tag, Ghost.reveal v));
+  let res = impl_serialize_tagged_none cbor_det_serialize_tag i1 c' out;
+  Trade.elim _ _;
+  res
+}
